feat: basic term `apply` and `Ord` instance

Cvc/Init/Basic.lean
@@ -18,30 +18,40 @@ export Lean (Rat)
 
 
 
+
 /-! ## Re-exports from `cvc5` -/
 
 inductive Error : Type u
 | internal (msg : String)
+| unsupported (msg : String)
 | userError (msg : String)
+deriving Inhabited
 
 namespace Error
 
 def toCvc5 : Error → cvc5.Error
 | .internal "a value is missing" => .missingValue
 | .internal msg => .error msg
+| .unsupported msg => .unsupported msg
 | .userError msg => .error msg
 
 def ofCvc5 : cvc5.Error → Error
 | .missingValue => .internal "a value is missing"
-| .error msg => .userError s!"{msg}"
-| .option msg => .userError s!"option error: {msg}"
-| .unsupported msg => .userError s!"unsupported: {msg}"
-| .recoverable msg => .userError s!"recoverable: {msg}"
+| .error msg => .internal s!"{msg}"
+| .option msg => .internal s!"option error: {msg}"
+| .unsupported msg => .unsupported msg
+| .recoverable msg => .internal s!"recoverable: {msg}"
+
+instance : MonadLift (Except cvc5.Error) (Except Error) where
+  monadLift
+  | .ok res => .ok res
+  | .error e => .error (ofCvc5 e)
 
 instance : Coe cvc5.Error Error := ⟨ofCvc5⟩
 
 protected def toString : Error → String
 | .internal msg => "internal error: " ++ msg
+| .unsupported msg => "unsupported: " ++ msg
 | .userError msg => "user error: " ++ msg
 
 instance instToString : ToString Error :=
@@ -52,3 +62,153 @@ end Error
 
 
 /-! ## Helpers -/
+
+
+
+structure ArrayMin (n : Nat) (α : Type u) : Type u where
+mk' ::
+  pref : Array α
+  inv : pref.size = n := by rfl
+  suff : Array α := #[]
+deriving Hashable
+
+namespace ArrayMin
+
+instance [Inhabited α] : Inhabited (ArrayMin n α) where
+  default := ⟨Array.mkArray n default, by simp, #[]⟩
+
+def mk (pref : Array α) (suff : Array α := #[]) : ArrayMin pref.size α :=
+  ⟨pref, rfl, suff⟩
+
+protected def toString [ToString α] (self : ArrayMin n α) : String :=
+  if self.suff.isEmpty then
+    toString self.pref
+  else
+    s!"{self.pref}{self.suff}"
+
+instance [ToString α] : ToString (ArrayMin n α) := ⟨ArrayMin.toString⟩
+
+
+variable (self : ArrayMin n α)
+
+@[simp]
+theorem pref_size : self.pref.size = n :=
+  self.inv
+
+abbrev size : Nat := n + self.suff.size
+
+@[simp]
+theorem min_le_size : n ≤ self.size := by
+  simp only [Nat.le_add_right]
+
+def get : (i : Fin self.size) → α
+| ⟨i, h_i⟩ =>
+  if h : i < n then
+    self.pref.get ⟨i, by simp only [pref_size, h]⟩
+  else
+    let h' : i - n < self.suff.size := by
+      simp [size] at h_i
+      exact Nat.sub_lt_left_of_lt_add (Nat.le_of_not_lt h) h_i
+    self.suff.get ⟨i - n, by simp only [pref_size, h']⟩
+
+instance instGetElem : GetElem (ArrayMin n α) Nat α (fun arr i => i < arr.size) where
+  getElem self i h_i := self.get ⟨i, h_i⟩
+
+def get? (self : ArrayMin n α) (i : Nat) : Option α :=
+  if h : i < self.size
+  then self.get ⟨i, h⟩
+  else none
+
+def get! [Inhabited α] (self : ArrayMin n α) (i : Nat) : α :=
+  if let some a := self.get? i
+  then a
+  else panic! s!"illegal index {i} for `ArrayMin {n} _` of size {self.size}"
+
+def getN (i : Nat) (h : i < n := by decide) : α :=
+  self.pref.get ⟨i, by simp [h]⟩
+
+def toArray : Array α := self.pref ++ self.suff
+
+def toList : List α := self.pref.data ++ self.suff.data
+
+def push (a : α) : ArrayMin n α :=
+  {self with suff := self.suff.push a }
+
+def drainFirst : ArrayMin n.succ α → α × ArrayMin n α
+| ⟨⟨fst::pref⟩, h_pref', suff⟩ =>
+  (fst, ⟨
+    ⟨pref⟩,
+    by
+      simp at h_pref'
+      assumption,
+    suff
+  ⟩)
+
+instance instForIn : ForIn m (ArrayMin n α) α where
+  forIn self init f := do
+    let mut acc := init
+    for a in self.pref do
+      match ← f a acc with
+      | .done a => return a
+      | .yield a => acc := a
+    for a in self.suff do
+      match ← f a acc with
+      | .done a => return a
+      | .yield a => acc := a
+    return acc
+
+structure Frame (n : Nat) (α : Type u) : Type u where
+private mk ::
+  private pref : Array α := #[]
+  private suff : Array α := #[]
+deriving Inhabited
+
+namespace Frame
+def new (n : Nat) : Frame n α :=
+  ⟨#[], #[]⟩
+
+variable (self : Frame n α)
+
+def push (a : α) : Frame n α :=
+  if self.pref.size < n then
+    {self with pref := self.pref.push a}
+  else
+    {self with suff := self.suff.push a}
+
+def finalize [Inhabited α] : ArrayMin n α :=
+  if h : self.pref.size = n then
+    ⟨self.pref, h, self.suff⟩
+  else
+    panic! s!"[ArrayMin.finalize] unexpected prefix of size {self.pref.size}, expected {n}"
+end Frame
+
+def newFrame : ArrayMin n α → Frame n β
+| _ => Frame.new n
+
+structure Iter (n : Nat) (α : Type u) : Type u where
+private mk ::
+  val : ArrayMin n α
+  pos : Nat
+
+namespace Iter
+variable (self : Iter n α)
+
+abbrev isNotDone : Bool :=
+  self.pos < self.val.size
+abbrev isDone : Bool :=
+  ¬ self.isNotDone
+
+def next? : Option α × Iter n α :=
+  if h : self.isNotDone then
+    let next := self.val.get ⟨
+      self.pos,
+      by simp [isNotDone] at h ; simp [h]
+    ⟩
+    (next, {self with pos := self.pos.succ})
+  else (none, self)
+end Iter
+
+def iter : Iter n α :=
+  ⟨self, 0⟩
+
+end ArrayMin
